Finish Ass 12, reviewed assignments & materials

sf/Assignment12_05.v
@@ -12,32 +12,61 @@ Require Export Assignment12_04.
 >>
 *)
 
+Notation x := (Id 0).
+Notation f := (Id 1).
+
 Definition halve : tm :=
-  FILL_IN_HERE.
+  tfix (tabs f (TArrow TNat TNat) (tabs x TNat (tif0 (tvar x) (tnat 0) (tif0 (tpred (tvar x)) (tnat 0) (tsucc (tapp (tvar f) (tpred (tpred (tvar x))))))))).
 
 Example halve_type: empty |- halve \in TArrow TNat TNat.
 Proof.
   (* unfold halve; eauto 10. *)
-  exact FILL_IN_HERE.
+  unfold halve; eauto 10.
 Qed.
 
 Example halve_10: tapp halve (tnat 10) ==>* tnat 5.
 Proof.
   (* unfold halve; normalize. *)
-  exact FILL_IN_HERE.
+  unfold halve; normalize.
 Qed.
 
 Example halve_11: tapp halve (tnat 11) ==>* tnat 5.
 Proof.
   (* unfold halve; normalize. *)
-  exact FILL_IN_HERE.
+  unfold halve; normalize.
 Qed.
 
+Lemma multi_succ_congru: forall t t',
+  t ==>* t' -> tsucc t ==>* tsucc t'.
+Proof.
+  intros. induction H.
+  - apply multi_refl.
+  - apply multi_step with (tsucc y). apply ST_Succ1. assumption. assumption.
+Qed.
+
+Lemma multi_succ: forall t n,
+  t ==>* tnat n -> tsucc t ==>* tnat (S n).
+Proof.
+  intros. eapply multi_trans with (tsucc (tnat n)).
+  apply multi_succ_congru. assumption. (* induction H; eauto. *)
+  eapply multi_step. apply ST_SuccNat. apply multi_refl.
+Qed.
 
 Theorem halve_correct: forall n,
    tapp halve (tnat (n+n)) ==>* tnat n.
 Proof.
-  exact FILL_IN_HERE.
+  induction n.
+  - unfold halve. normalize.
+  - unfold halve in *. simpl. rewrite plus_comm. simpl.
+    eapply multi_step. apply ST_AppFix; auto.
+    eapply multi_step. apply ST_App1. auto. simpl.
+    eapply multi_step. apply ST_AppAbs. auto. simpl.
+    eapply multi_step. apply ST_If0Nonzero.
+    eapply multi_step. apply ST_If01. apply ST_PredNat. simpl.
+    eapply multi_step. apply ST_If0Nonzero.
+    eapply multi_step. apply ST_Succ1. apply ST_App2. auto. apply ST_Pred. apply ST_PredNat. simpl.
+    eapply multi_step. apply ST_Succ1. apply ST_App2. auto. apply ST_PredNat. simpl.
+    apply multi_succ. assumption.
 Qed.
 
 (*-- Check --*)
