sf/Assignment09_09.v
@@ -46,17 +46,21 @@ Theorem factorial_dec_correct: forall m,
   {{ fun st => st Y = fact m }}.
 Proof.
   intros.
-  eapply hoare_consequence_post. apply hoare_seq with (fun st => st Y * fact (st X) = fact m).
-  apply hoare_while. apply hoare_seq with ((fun st => st Y * fact (st X) = fact m)[X |-> (AMinus (AId X) (ANum 1))]). apply hoare_asgn.
+  apply hoare_seq with (fun st => st Y * fact (st X) = fact m).
+  eapply hoare_consequence_post. apply hoare_while.
+  eapply hoare_seq. apply hoare_asgn.
   eapply hoare_consequence_pre. apply hoare_asgn.
-  intros st H. destruct H. simpl in H0. apply negb_true in H0. apply beq_nat_false in H0.
-  unfold assn_sub, update. simpl. assert (st X * fact (st X - 1) = fact (st X)).
+  unfold assert_implies, assn_sub, update. simpl. intros.
+  destruct H. apply negb_true in H0. apply beq_nat_false in H0. rewrite <- H.
+  assert (st X * fact (st X - 1) = fact (st X)).
   induction (st X). tauto. simpl. rewrite <- minus_n_O. reflexivity.
-  rewrite <- H. rewrite <- mult_assoc. rewrite H1. reflexivity.
+  rewrite <- mult_assoc. rewrite H1. reflexivity.
+  unfold assert_implies, assn_sub, update. simpl. intros.
+  destruct H. apply negb_false in H0. apply beq_nat_true in H0. rewrite <- H.
+  rewrite H0. simpl. omega.
   eapply hoare_consequence_pre. apply hoare_asgn.
-  unfold assert_implies, assn_sub, update. simpl. intros. rewrite H. omega.
-  intros st H. destruct H. simpl in H0. apply negb_false in H0. apply beq_nat_true in H0.
-  rewrite H0 in H. simpl in H. rewrite <- H. omega.
+  unfold assert_implies, assn_sub, update. simpl. intros.
+  rewrite H. omega.
 Qed.
 
 (*-- Check --*)
