sf/Assignment09_10.v
@@ -64,26 +64,27 @@ Theorem add_three_numbers_correct: forall a b c,
   END
   {{ fun st => st Z = a + b + c }}.
 Proof.
-  intros.
-  eapply hoare_consequence_post.
-  apply hoare_seq with ((fun st => st Z = st X + c /\ st Y = 0) [Z |-> ANum c][Y |-> ANum 0]).
-  apply hoare_seq with ((fun st => st Z = st X + c /\ st Y = 0)[Z |-> ANum c]).
+  intros. eapply hoare_seq. eapply hoare_seq.
   apply hoare_seq with (fun st => st Z = st X + c /\ st Y = 0).
   apply hoare_seq with (fun st => st Z = st Y + a + c).
-  apply hoare_while. eapply hoare_consequence_pre. eapply hoare_seq.
-  apply hoare_asgn. apply hoare_asgn.
-  intros st H. destruct H. simpl in H0. apply negb_true in H0. apply beq_nat_false in H0.
-  unfold assn_sub, update. simpl. omega.
-  eapply hoare_consequence_post.
-  apply hoare_while. eapply hoare_consequence_pre. eapply hoare_seq.
-  apply hoare_asgn. apply hoare_asgn.
-  intros st H. destruct H. simpl in H0. apply negb_true in H0. apply beq_nat_false in H0.
-  unfold assn_sub, update. simpl. omega.
-  intros st H. destruct H. destruct H. simpl in H0. apply negb_false in H0. apply beq_nat_true in H0. omega.
+  eapply hoare_consequence_post. apply hoare_while.
+  eapply hoare_seq. apply hoare_asgn.
+  eapply hoare_consequence_pre. apply hoare_asgn.
+  unfold assert_implies, assn_sub, update. simpl. intros. destruct H.
+  apply negb_true in H0. apply beq_nat_false in H0. omega.
+  unfold assert_implies, assn_sub, update. simpl. intros. destruct H.
+  apply negb_false in H0. apply beq_nat_true in H0. omega.
+  eapply hoare_consequence_post. apply hoare_while.
+  eapply hoare_seq. apply hoare_asgn.
+  eapply hoare_consequence_pre. apply hoare_asgn.
+  unfold assert_implies, assn_sub, update. simpl. intros. destruct H.
+  destruct H. apply negb_true in H0. apply beq_nat_false in H0. omega.
+  unfold assert_implies, assn_sub, update. simpl. intros. destruct H.
+  destruct H. apply negb_false in H0. apply beq_nat_true in H0. omega.
   apply hoare_asgn. apply hoare_asgn.
   eapply hoare_consequence_pre. apply hoare_asgn.
-  intros st H. unfold assn_sub, update. simpl. omega.
-  intros st H. destruct H. simpl in H0. apply negb_false in H0. apply beq_nat_true in H0. omega.
+  unfold assert_implies, assn_sub, update. simpl. intros. destruct H.
+  split; omega.
 Qed.
 
 (*-- Check --*)
