sf/Assignment10_06.v
@@ -18,9 +18,7 @@ Proof.
     + apply IHP11.
       * assumption.
       * assert (y = y0). eapply step_deterministic_alt. apply H. apply H0. subst.
-        inversion P21; subst. clear H0. rename y0 into y. assumption.
-        rename y0 into y1. assert (y = y1). eapply step_deterministic_alt. apply H2. apply H0.
-        subst. assumption.
+        assumption.
       * assumption.
 Qed.
 
