sf/Assignment10_16.v
@@ -20,7 +20,7 @@ Proof.
   intros; induction c; eauto; right.
   - remember (aexp_strong_progress st a) as Ha; clear HeqHa;
     destruct Ha as [[? ?] | [? ?]]; subst; eauto.
-  - destruct IHc1 as [ | [? [? ?]]]; subst. eauto. eauto.
+  - destruct IHc1 as [ | [? [? ?]]]; subst; eauto.
   - remember (bexp_strong_progress st b) as Hb; clear HeqHb;
     destruct Hb as [[? | ?] | [? ?]]; subst; eauto.
   - destruct IHc1 as [ | [? [? ?]]]; destruct IHc2 as [ | [? [? ?]]]; subst; eauto.
