sf/Assignment12_02.v
@@ -7,7 +7,8 @@ Corollary typable_empty__closed : forall t T,
     empty |- t \in T  ->
     closed t.
 Proof.
-  exact FILL_IN_HERE.
+  intros t T H x Hc. apply free_in_context with (T:=T) (Gamma:=\empty) in Hc.
+  solve by inversion 2. assumption.
 Qed.
 
 (*-- Check --*)
