sf/Assignment12_06.v
@@ -2,10 +2,51 @@ Require Export Assignment12_05.
 
 (* problem #06: 10 points *)
 
+Lemma tloop_back: exists p q, tapp tloop (tnat 0) ==> p /\ p ==> q /\ q ==> tapp tloop (tnat 0).
+  eexists. eexists. unfold tloop. split.
+  - eauto.
+  - split.
+    + eauto.
+    + simpl. constructor. constructor.
+Qed.
+
+Theorem MoreStlc_value_is_nf: forall v t,
+  value v -> v ==> t -> False.
+Proof with eauto.
+  intros; generalize dependent t; assert (normal_form step v)...
+  unfold normal_form; intros; induction H; intros contra; destruct contra;
+  try solve by inversion; try inversion H0; try inversion H1; subst...
+Qed.
+
+Hint Resolve MoreStlc_value_is_nf.
+
+Theorem MoreStlc_deterministic:
+  deterministic step.
+Proof with eauto.
+  unfold deterministic; intros; generalize dependent y2;
+  induction H as [| |? ? ? ? P| | | | | |? ? ? ? P| | | | | |? ? ? ? P| |? ? ? P|
+  |? ? ? P| | | | | | | | |? ? ? ? P| | | ? ? ? ? ? ? P| |? ? ? P]; intros;
+  inversion H0; subst; try solve by inversion;
+  try replace t0'0 with t0';
+  try replace t1'0 with t1';
+  try replace t2'0 with t2';
+  eauto; exfalso...
+Qed.
+
 Theorem tloop_diverges:
   ~ exists t, tapp tloop (tnat 0) ==>* t /\ normal_form step t.
 Proof.
-  exact FILL_IN_HERE.
+  intros Hc. destruct Hc as [t H]. destruct H.
+  remember tloop_back. clear Heqe. destruct e as [p [q [H1 [H2 H3]]]].
+  unfold normal_form in H0. apply H0. clear H0.
+  generalize dependent p. generalize dependent q.
+  induction H; intros. exists p. assumption.
+  inversion H0; subst. remember MoreStlc_deterministic. unfold deterministic in d.
+  assert (p = z). eapply d. apply H1. apply H. subst.
+  eapply IHmulti. apply H. apply H2. apply H3. 
+  remember MoreStlc_deterministic; unfold deterministic in d.
+  assert (y = p). eapply d. apply H. apply H1. subst.
+  eapply IHmulti. apply H. apply H2. apply H3.
 Qed.
 
 (*-- Check --*)
